simplified and finished dpll

dpll.v
@@ -82,7 +82,205 @@ Eval compute in dpll numVars f3.
 
 
 (*=============================================================================
- * semantics
+ * logic utility
+ *===========================================================================*)
+
+Lemma dnc : forall p : Prop, ~~ (p \/ ~p).
+  tauto.
+Qed.
+
+
+(*=============================================================================
+ * dpll facts
+ *===========================================================================*)
+
+Lemma getVal_Some : forall m n, n < length m -> getVal m n = Some (nth n m true).
+  induction m; simpl; intros; try omega.
+  destruct n; auto.
+  apply IHm; omega.
+Qed.
+
+Lemma getVal_None : forall n m, length m <= n -> getVal m n = None.
+  induction n; destruct m; simpl; auto; try omega; intros.
+  apply IHn; omega.
+Qed.
+
+Lemma okLit_false_lt : forall s l, okLit s l = false -> litVar l < length s.
+  unfold okLit; intros.
+  destruct (getVal s (litVar l)) eqn:?; try congruence.
+  destruct (le_lt_dec (length s) (litVar l)); auto.
+  solve [rewrite getVal_None in * by auto; congruence].
+Qed.
+Hint Resolve okLit_false_lt.
+
+Lemma okClause_In : forall s c l, okClause s c = false -> In l c
+                                  -> okLit s l = false.
+  induction c; simpl; try tauto; intros.
+  destruct (okLit s a) eqn:?; try congruence.
+  destruct H0; subst; auto.
+Qed.
+Hint Resolve okClause_In.
+
+
+(*=============================================================================
+ * denotational satisfiablity
+ *===========================================================================*)
+
+Definition context := nat -> Prop.
+
+Section denoteSat.
+  Variable g : context.
+
+  Definition satLit l :=
+    match l with
+      | pos n => g n
+      | neg n => ~ g n
+    end.
+
+  Definition satClause c := exists l, In l c /\ satLit l.
+
+  Definition satFormula f := forall c, In c f -> satClause c.
+End denoteSat.
+
+
+(*=============================================================================
+ * refutaional proofs
+ *===========================================================================*)
+
+Inductive refutable (F : formula) (l : list bool) : Prop :=
+| refutable_base  : okFormula l F = false -> refutable F l
+| refutable_split : refutable F (l ++ true :: nil)
+                    -> refutable F (l ++ false :: nil) -> refutable F l.
+
+Hint Constructors refutable.
+
+Lemma dpll_h_refutable : forall n f l, dpll_h f l n = None -> refutable f l.
+  induction n; simpl; intros.
+  {
+    destruct (okFormula l f) eqn:?; try congruence; auto.
+  }
+  {
+    destruct (okFormula l f) eqn:?; auto.
+    destruct (dpll_h f (l ++ true :: nil) n) eqn:?; try congruence; auto.
+  }
+Qed.
+
+Lemma dpll_refutable : forall n f, dpll n f = None -> refutable f nil.
+  intros; eapply dpll_h_refutable; eauto 2.
+Qed.
+
+
+(*=============================================================================
+ * m2i - turn a finite model into a total interpretation function
+ *===========================================================================*)
+
+Definition m2i m n := nth n m true.
+
+Lemma m2i_app_lt : forall x y v, v < length x -> m2i (x ++ y) v = m2i x v.
+  unfold m2i; intros.
+  rewrite app_nth1; auto.
+Qed.
+
+Lemma m2i_app_ge : forall x y v, v >= length x
+                                 -> m2i (x ++ y) v = m2i y (v - length x).
+  unfold m2i; intros.
+  rewrite app_nth2; auto.
+Qed.
+
+Lemma getVal_m2i : forall m n, n < length m -> getVal m n = Some (m2i m n).
+  unfold m2i; apply getVal_Some; auto.
+Qed.
+
+
+(*=============================================================================
+ * refutable ==> unsat (denotational)
+ *===========================================================================*)
+
+Definition assumed (g : context) m
+  := forall v, v < length m -> if m2i m v then g v else ~ g v.
+
+Hint Resolve in_eq in_cons.
+
+Lemma okClause_false : forall g s x, okClause s x = false -> assumed g s
+                                     -> ~ satClause g x.
+  intros; red; destruct 1 as [? [] ].
+  assert (okLit s x0 = false) by eauto 3.
+  assert (litVar x0 < length s) by auto.
+  specialize (H0 _ H4).
+  unfold okLit in *; rewrite getVal_m2i in * by auto.
+  destruct x0; simpl in *.
+  solve [rewrite H3 in *; tauto].
+  solve [apply Bool.negb_false_iff in H3; rewrite H3 in *; tauto].
+Qed.
+Hint Resolve okClause_false.
+
+Lemma okFormula_false : forall s g f, okFormula s f = false -> assumed g s
+                                      -> ~ satFormula g f.
+  induction f; simpl; try congruence; intros.
+  destruct (okClause s a) eqn:?.
+  {
+    intro.
+    eelim IHf; eauto 3.
+    red; auto.
+  }
+  intro.
+  assert (satClause g a) by auto.
+  contradict H2; eauto 3.
+Qed.
+Hint Resolve okFormula_false.
+
+Lemma assume_add_true : forall g l, assumed g l -> g (length l)
+                                    -> assumed g (l ++ true :: nil).
+  red; intros.
+  destruct (le_lt_dec (length l) v).
+  {
+    rewrite m2i_app_ge; auto.
+    assert (length l = v).
+    solve [autorewrite with list in *; simpl in *; omega].
+    rewrite H2; simpl.
+    replace (v - v) with 0 by omega; simpl; congruence.
+  }
+  {
+    rewrite m2i_app_lt by auto; apply H; auto.
+  }
+Qed.
+Hint Resolve assume_add_true.
+
+Lemma assume_add_false : forall g l, assumed g l -> ~ g (length l)
+                                     -> assumed g (l ++ false :: nil).
+  red; intros.
+  destruct (le_lt_dec (length l) v).
+  {
+    rewrite m2i_app_ge; auto.
+    assert (length l = v).
+    solve [autorewrite with list in *; simpl in *; omega].
+    rewrite H2; simpl.
+    replace (v - v) with 0 by omega; simpl; congruence.
+  }
+  {
+    rewrite m2i_app_lt by auto; apply H; auto.
+  }
+Qed.
+Hint Resolve assume_add_false.
+
+Lemma refutable_unsat_h : forall g f s, refutable f s -> assumed g s
+                                      -> ~ satFormula g f.
+  induction 1; intros; eauto 3.
+  intro; elim (@dnc (g (length l))); red; destruct 1; contradict H2; auto.
+Qed.
+
+Lemma refutable_unsat : forall g f, refutable f nil -> ~ satFormula g f.
+  intros; eapply refutable_unsat_h; eauto 3.
+  red; simpl; intros; omega.
+Qed.
+
+Lemma dpll_unsat_sound : forall n g f, dpll n f = None -> ~ satFormula g f.
+  intros; eapply refutable_unsat, dpll_refutable; eauto 2.
+Qed.
+
+
+(*=============================================================================
+ * clssical semantics
  *===========================================================================*)
 
 Definition interp := nat -> bool.
@@ -101,16 +299,10 @@ Definition interpFormula (I : interp) (f : formula) :=
 
 Definition satisfiable f := exists i, interpFormula i f = true.
 
-Definition entails f c := forall i, interpFormula i f = true
-                                    -> interpClause i c = true.
-
 
 (*=============================================================================
  * semantics tests
  *===========================================================================*)
-
-Example I n := match n with 0 => false | 1 => true | _ => true end.
-Eval simpl in interpLit I (pos 0).
 
 Goal forall (i : interp), interpClause i nil = false.
   simpl; auto.
@@ -129,6 +321,55 @@ Goal forall (i : interp), interpFormula i (c1 :: c2 :: nil) = false.
   simpl; intros.
   destruct (i 3) eqn:?; simpl; auto.
 Qed.
+
+Example I n := match n with 0 => false | 1 => true | _ => true end.
+Eval simpl in interpLit I (pos 0).
+
+
+(*=============================================================================
+ * denotational satisfiablity and classical satisfiability
+ *===========================================================================*)
+
+(* a trivial Coq context from classical Boolean model *)
+Definition i2g (i : interp) v := if i v then True else False.
+
+Lemma denoteLit_i2g : forall i l, interpLit i l = true -> satLit (i2g i) l.
+  destruct l; simpl; unfold i2g; intros;
+  destruct (i n); simpl in *; auto; congruence.
+Qed.    
+Hint Resolve denoteLit_i2g.
+
+Lemma satClause_i2g : forall i x, interpClause i x = true
+                                     -> satClause (i2g i) x.
+  induction x; simpl; try congruence; intros.
+  apply Bool.orb_true_iff in H; destruct H.
+  exists a; simpl; auto.
+  destruct IHx as [? [] ]; auto.
+  exists x0; simpl; auto.
+Qed.
+Hint Resolve satClause_i2g.
+
+Lemma satFormula_i2g : forall i x, interpFormula i x = true
+                                     -> satFormula (i2g i) x.
+  induction x; red; simpl; try tauto; intros.
+  apply Bool.andb_true_iff in H; destruct H.
+  destruct H0; subst; auto.
+  apply IHx; auto.
+Qed.
+Hint Resolve satFormula_i2g.
+
+Theorem satisfiable_satFormula : forall f, satisfiable f
+                                           -> exists g, satFormula g f.
+  destruct 1; exists (i2g x); auto.
+Qed.
+
+Corollary dpll_unsat_sound' : forall n f, dpll n f = None -> ~ satisfiable f.
+  red; intros; edestruct satisfiable_satFormula; eauto 2.
+  contradict H1; eapply dpll_unsat_sound; eauto 2.
+Qed.
+
+Goal forall g f, satFormula g f -> satisfiable f. (* hard to prove? *)
+Abort.
 
 
 (*=============================================================================
@@ -200,25 +441,8 @@ Hint Resolve wf_formula_cons_inv'.
 
 
 (*=============================================================================
- * dpll correctness (SAT case)
+ * dpll soundness (SAT case)
  *===========================================================================*)
-
-Lemma getVal_Some : forall m n, n < length m -> getVal m n = Some (nth n m true).
-  induction m; simpl; intros; try omega.
-  destruct n; auto.
-  apply IHm; omega.
-Qed.
-
-Lemma getVal_None : forall n m, length m <= n -> getVal m n = None.
-  induction n; destruct m; simpl; auto; try omega; intros.
-  apply IHn; omega.
-Qed.
-
-Definition m2i m n := nth n m true.
-
-Lemma getVal_m2i : forall m n, n < length m -> getVal m n = Some (m2i m n).
-  unfold m2i; apply getVal_Some; auto.
-Qed.
 
 Lemma okLit_interpLit : forall m a, okLit m a = true -> litVar a < length m
                                     -> interpLit (m2i m) a = true.
@@ -254,7 +478,7 @@ Lemma okFormula_interpFormula : forall nv m F, okFormula m F = true
   apply Bool.andb_true_iff; split; eauto 3.
 Qed.
 
-Ltac dpll :=
+Ltac options :=
   try match goal with
         | H: None = Some _ |- _ => inversion H
         | H: Some _ = None |- _ => inversion H
@@ -264,15 +488,15 @@ Ltac dpll :=
 Lemma dpll_h_okFormula : forall F n m m', dpll_h F m n = Some m'
                                           -> okFormula m' F = true.
   induction n; simpl; intros;
-  destruct (okFormula m F) eqn:?; dpll.
-  destruct (dpll_h F (m ++ true :: nil) n) eqn:?; dpll; eauto 3.
+  destruct (okFormula m F) eqn:?; options.
+  destruct (dpll_h F (m ++ true :: nil) n) eqn:?; options; eauto 3.
 Qed.
 
 Lemma dpll_h_length : forall F n m m', dpll_h F m n = Some m'
                                           -> length m' = length m + n.
   induction n; simpl; intros;
-  destruct (okFormula m F) eqn:?; dpll.
-  destruct (dpll_h F (m ++ true :: nil) n) eqn:?; dpll; eauto 3.
+  destruct (okFormula m F) eqn:?; options.
+  destruct (dpll_h F (m ++ true :: nil) n) eqn:?; options; eauto 3.
   {
     replace (length m + S n) with (length (m ++ true :: nil) + n); eauto.
     autorewrite with list; simpl; omega.
@@ -297,622 +521,51 @@ Theorem dpll_length : forall F nv m , dpll nv F = Some m
 Qed.
 Hint Resolve dpll_length.
 
-Theorem dpll_Some_sound : forall F m nv, dpll nv F = Some m -> wf_formula nv F
-                                         -> satisfiable F.
-  red; intros.
+Theorem dpll_Some_interp : forall nv F m, dpll nv F = Some m -> wf_formula nv F
+                                       -> interpFormula (m2i m) F = true.
+  intros.
   assert (length m = nv) by eauto 3.
-  exists (m2i m); eapply okFormula_interpFormula; try eassumption; eauto 3; omega.
+  eapply okFormula_interpFormula; try eassumption; eauto 3; omega.
 Qed.
 
-
-(*=============================================================================
- * if satsifiable, there exists a finite model.
- *===========================================================================*)
-
-Definition clamp f nv n := if lt_dec n nv then f n else true.
-
-Lemma clamp_eq_lt : forall n x i, x < n -> clamp i n x = i x.
-  unfold clamp; intros.
-  destruct (lt_dec x n); auto; tauto.
-Qed.
-
-Lemma interpLit_clamp : forall nv i x, litVar x < nv -> interpLit i x = true
-                                       -> interpLit (clamp i nv) x = true.
-  unfold interpLit; intros.
-  destruct x; rewrite clamp_eq_lt by auto; auto.
-Qed.
-Hint Resolve interpLit_clamp.
-
-Lemma interpClause_clamp : forall nv i c, wf_clause nv c
-                              -> interpClause i c = true
-                              -> interpClause (clamp i nv) c = true.
-  induction c; simpl; auto; intros.
-  apply Bool.orb_true_iff.
-  apply Bool.orb_true_iff in H0; destruct H0; eauto 4.
-Qed.
-Hint Resolve interpClause_clamp.
-  
-Lemma interpFormula_clamp : forall nv i F, wf_formula nv F
-                                -> interpFormula i F = true
-                                -> interpFormula (clamp i nv) F = true.
-  induction F; simpl; auto; intros.
-  apply Bool.andb_true_iff in H0; destruct H0.
-  apply Bool.andb_true_iff; split; eauto 3.
-Qed.
-Hint Resolve interpFormula_clamp.
-
-Lemma clamp_m2i : forall i n,
-                       exists m, length m = n /\ forall v, clamp i n v = m2i m v.
-  induction n; intros.
-  {
-    exists nil; simpl; auto.
-    split; auto; intros.
-    destruct v; auto.
-  }
-  {
-    destruct IHn as [? [] ].
-    exists (x ++ (i n) :: nil); intros.
-    autorewrite with list; simpl; split; try omega; intros.
-    specialize (H0 v).
-    unfold clamp, m2i in *; destruct (lt_dec v (S n)).
-    {
-      destruct (lt_dec v n).
-      {
-        rewrite H0; subst.
-        rewrite app_nth1; auto.
-      }
-      {
-        assert (v = n) by omega; subst.
-        rewrite app_nth2; auto.
-        replace (length x - length x) with 0 by omega.
-        simpl; auto.
-      }
-    }
-    {
-      destruct (lt_dec v n); try omega; subst.
-      rewrite app_nth2 by omega.
-      destruct (v - length x) eqn:?; try omega.
-      simpl.
-      destruct n; auto.
-    }
-  }
-Qed.
-
-Lemma interpLit_compat : forall x y l, (forall v, x v = y v)
-                             -> interpLit x l = true -> interpLit y l = true.
-  unfold interpLit; intros; auto.
-  destruct l; rewrite <- H; auto.
-Qed.
-Hint Resolve interpLit_compat.
-
-Lemma interpClause_compat : forall x y c, (forall v, x v = y v)
-                              -> interpClause x c = true
-                              -> interpClause y c = true.
-  induction c; simpl; auto; intros.
-  apply Bool.orb_true_iff in H0.
-  destruct H0; apply Bool.orb_true_iff; eauto 3.
-Qed.
-Hint Resolve interpClause_compat.
-
-Lemma interpFormula_compat : forall x y F, (forall v, x v = y v)
-                                 -> interpFormula x F = true
-                                 -> interpFormula y F = true.
-  induction F; simpl; auto; intros.
-  apply Bool.andb_true_iff in H0; destruct H0.
-  apply Bool.andb_true_iff; split; eauto 3.
-Qed.  
-Hint Resolve interpFormula_compat.
-
-Lemma satisfiable_model : forall nv F, wf_formula nv F -> satisfiable F
-                  -> exists m, interpFormula (m2i m) F = true /\ length m = nv.
-  destruct 2.
-  assert (interpFormula (clamp x nv) F = true) by auto.
-  destruct (clamp_m2i x nv) as [? [] ]; eauto 4.
-Qed.
-
-
-(*=============================================================================
- * dpll correctness (UNSAT case)
- *===========================================================================*)
-
-Lemma okLit_interpLit' : forall m x, okLit m x = false
-                                     -> interpLit (m2i m) x = false.
-  unfold okLit; intros.
-  destruct (le_lt_dec (length m) (litVar x)).
-  rewrite getVal_None in * by auto; congruence.
-  rewrite getVal_m2i in * by auto; auto.
-  destruct x; simpl in *; auto.
-Qed.
-Hint Resolve okLit_interpLit'.
-
-Lemma okClause_interpClause' : forall m x, okClause m x = false
-                                           -> interpClause (m2i m) x = false.
-  induction x; simpl; auto; intros.
-  apply Bool.orb_false_iff.
-  destruct (okLit m a) eqn:?; try congruence; auto.
-Qed.
-Hint Resolve okClause_interpClause'.
-
-Lemma okFormula_interpFormula' : forall m F, okFormula m F = false
-                                             -> interpFormula (m2i m) F = false.
-  induction F; simpl; auto; intros.
-  apply Bool.andb_false_iff.
-  destruct (okClause m a) eqn:?; auto.
-Qed.
-Hint Resolve okFormula_interpFormula'.
-
-
-Lemma okLit_app : forall b m x, okLit m x = false
-                                -> okLit (m ++ b :: nil) x = false.
-  unfold okLit; simpl; intros.
-  destruct (le_lt_dec (length m) (litVar x)).
-  rewrite getVal_None in * by auto; congruence.
-  rewrite getVal_Some in * by (autorewrite with list; omega).
-  destruct x; simpl in *; rewrite app_nth1 by auto; auto.
-Qed.
-Hint Resolve okLit_app.
-
-Lemma okClause_app : forall b m x, okClause m x = false
-                                   -> okClause (m ++ b :: nil) x = false.
-  induction x; simpl; auto; intros.
-  destruct (okLit m a) eqn:?; try congruence; auto.
-  destruct (okLit (m ++ b :: nil) a) eqn:?; auto.
-  assert (okLit (m ++ b :: nil) a = false) by auto; congruence.
-Qed.
-Hint Resolve okClause_app.
-
-Lemma okFormula_app : forall b m F, okFormula m F = false
-                                    -> okFormula (m ++ b :: nil) F = false.
-  induction F; simpl; auto; intros.
-  destruct (okClause m a) eqn:?, (okClause (m ++ b :: nil) a) eqn:?; auto.
-  assert (okClause (m ++ b :: nil) a = false) by auto; congruence.
-Qed.
-Hint Resolve okFormula_app.
-
-Lemma okFormua_app' : forall F x m, okFormula m F = false
-                                    -> okFormula (m ++ x) F = false.
-  induction x; simpl; intros; autorewrite with list; auto.
-  replace (m ++ a :: x) with ((m ++ a :: nil) ++ x)
-    by (rewrite <- app_assoc; simpl; auto); auto.
-Qed.
-Hint Resolve okFormua_app'.
-
-Lemma dpll_h_None : forall n m x F, dpll_h F m n = None -> length x = n
-                     -> okFormula (m ++ x) F = false.
-  induction n; simpl; intros.
-  {
-    destruct (okFormula m F) eqn:?; dpll.
-  }
-  {
-    destruct (okFormula m F) eqn:?; dpll.
-    destruct (dpll_h F (m ++ true :: nil) n) eqn:?; dpll.
-    destruct x; simpl in *; try omega.
-    replace (m ++ b :: x) with ((m ++ b :: nil) ++ x)
-      by (rewrite <- app_assoc; simpl; auto).
-    destruct b; auto.
-  }
-Qed.
-
-Lemma dpll_None : forall nv m F, dpll nv F = None -> length m = nv
-                               -> okFormula m F = false.
-  intros.
-  replace m with (nil ++ m) by auto.
-  eapply dpll_h_None; eauto.
-Qed.
-  
-Lemma dpll_None' : forall nv F m, dpll nv F = None -> length m = nv
-                    -> interpFormula (m2i m) F = false.
-  intros.
-  apply okFormula_interpFormula'.
-  eapply dpll_None; eauto 3.
-Qed.
-
-Theorem dpll_None_sound : forall nv F, dpll nv F = None -> wf_formula nv F
-                                       -> ~ satisfiable F.
+Theorem dpll_sat_sound : forall F nv, dpll nv F <> None -> wf_formula nv F
+                                     -> satisfiable F.
   red; intros.
-  edestruct satisfiable_model as [? [] ]; eauto 3.
-  assert (interpFormula (m2i x) F = false).
-  solve [eapply dpll_None'; eauto 3; omega].
-  congruence.
+  destruct (dpll nv F) eqn:?; try congruence.
+  exists (m2i l); eapply dpll_Some_interp; eauto 3.
+Qed.
+
+Corollary dpll_sat_sound' : forall n f, dpll n f <> None -> wf_formula n f
+                                       -> exists g, satFormula g f.
+  intros; eapply satisfiable_satFormula, dpll_sat_sound; eauto 3.
 Qed.
 
 
 (*=============================================================================
- * maxVarsFormula and well-formedness
+ * denotation into Coq (for reflexive tactics)
  *===========================================================================*)
 
-Fixpoint maxVarsClause c :=
-  match c with
-    | nil => 0
-    | l :: c' => max (litVar l) (maxVarsClause c')
-  end.
-
-Fixpoint maxVarsFormula F :=
-  match F with
-    | nil => 0
-    | c :: F' => max (maxVarsClause c) (maxVarsFormula F')
-  end.
-
-Lemma maxVarsClause_wf_clause : forall n x, maxVarsClause x < n -> wf_clause n x.
-  induction x; simpl; red; simpl; try tauto; intros.
-  apply NPeano.Nat.max_lub_lt_iff in H; destruct H.
-  destruct H0; subst; try tauto.
-  apply IHx; auto.
-Qed.
-Hint Resolve maxVarsClause_wf_clause.
-
-Lemma maxVarsFormula_In : forall F c n, maxVarsFormula F < n -> In c F
-                                            -> maxVarsClause c < n.
-  induction F; simpl; try tauto; destruct 2; subst;
-  apply NPeano.Nat.max_lub_lt_iff in H; destruct H; auto.
-Qed.
-Hint Resolve maxVarsFormula_In.
-
-Lemma maxVarsFormula_lt_wf : forall n F, maxVarsFormula F < n -> wf_formula n F.
-  red; intros; eauto 3.
-Qed.
-
-Theorem wf_maxVarsFormula : forall F, wf_formula (1 + maxVarsFormula F) F.
-  intros; apply maxVarsFormula_lt_wf; omega.
-Qed.
-Hint Resolve wf_maxVarsFormula.
-
-
-(*=============================================================================
- * conjecture : stronger theorem
- *===========================================================================*)
-
-Conjecture conj : forall F n, dpll n F = None
-                              -> dpll (1 + maxVarsFormula F) F = None.
-
-Lemma satisfiable_model' : forall F, satisfiable F
-                             -> exists m, interpFormula (m2i m) F = true
-                                          /\ length m = 1 + maxVarsFormula F.
-  destruct 1.
-  assert (wf_formula (1 + maxVarsFormula F) F) by auto.
-  assert (interpFormula (clamp x (1 + maxVarsFormula F)) F = true) by auto.
-  destruct (clamp_m2i x (1 + maxVarsFormula F)) as [? [] ]; eauto 4.
-Qed.
-
-Theorem dpll_None_sound' : forall n F, dpll n F = None
-                                       -> ~ satisfiable F.
-  red; intros.
-  assert (dpll (1 + maxVarsFormula F) F = None).
-  solve [eapply conj; eauto 3].
-  edestruct satisfiable_model' as [? [] ]; eauto 3.
-  assert (wf_formula (1 + maxVarsFormula F) F) by auto.
-  assert (interpFormula (m2i x) F = false).
-  solve [eapply dpll_None'; eauto 3].
-  congruence.
-Qed.
-
-
-(*=============================================================================
- * sublist
- *===========================================================================*)
-
-Section sublist.
-
-  Ltac e := eauto 3 with list.
-
-  Local Hint Constructors Forall : list.
-  Local Hint Resolve in_or_app Forall_impl : list.
-
-  Variable A : Type.
-
-  Definition sublist (x y : list A) := List.Forall (fun a => In a y) x.
-
-  Lemma sublist_refl : forall (x : list A), sublist x x.
-    unfold sublist; induction x; e.
-    constructor; simpl; e.
-    eapply Forall_impl; try eassumption; e.
-  Qed.
-
-  Lemma sublist_app : forall (l x y : list A), sublist l x \/ sublist l y
-                                                 -> sublist l (x ++ y).
-    induction l.
-    {
-      unfold sublist; simpl; intros; e.
-    }
-    {
-      unfold sublist; simpl; intros.
-      constructor.
-      destruct H; inversion_clear H; e.
-      apply IHl.
-      destruct H; inversion_clear H; e.
-    }
-  Qed.
-
-  Lemma sublist_In : forall x (a : A) y, sublist x y -> In a x -> In a y.
-    induction x; simpl; try tauto; inversion_clear 1; destruct 1; subst; auto.
-  Qed.
-
-End sublist.
-
-Local Hint Resolve sublist_refl sublist_app sublist_In.
-
-
-(*=============================================================================
- * interp facts
- *===========================================================================*)
-
-Lemma interpClause_exists : forall i x, interpClause i x = true
-                             -> exists l, In l x /\ interpLit i l = true.
-  induction x; simpl; try congruence; intros.
-  destruct (interpLit i a) eqn:?; eauto; simpl in *.
-  destruct IHx as [? [] ]; eauto.
-Qed.
-
-Lemma interpClause_In : forall l i x, interpLit i l = true -> In l x
-                                      -> interpClause i x = true.
-  induction x; simpl; try tauto; intros.
-  destruct H0; subst.
-  rewrite H; auto.
-  destruct (interpLit i a) eqn:?; eauto; simpl in *.
-Qed.
-
-Lemma interpClause_In' : forall x i l, interpClause i x = false
-                           -> In l x -> interpLit i l = false.
-  induction x; simpl; try tauto; intros.
-  eapply Bool.orb_false_iff in H; destruct H.
-  destruct H0; subst; auto.
-Qed.
-
-Hint Resolve interpClause_In interpClause_In'.
-
-Lemma interpClause_sublist : forall i x y, interpClause i x = true
-                               -> sublist x y -> interpClause i y = true.
-  intros.
-  edestruct interpClause_exists as [? [] ]; try eassumption.
-  eapply interpClause_In; try eassumption.
-  eapply Forall_forall in H0; eassumption.
-Qed.
-
-Lemma interpClause_sublist' : forall i x y, interpClause i y = false
-                                -> sublist x y -> interpClause i x = false.
-  induction x; simpl; intros; auto.
-  apply Bool.orb_false_iff.
-  inversion_clear H0; eauto 4.
-Qed.
-
-Hint Resolve interpClause_sublist interpClause_sublist'.
-
-Lemma interpClause_app : forall i x y,
-                           interpClause i x = true \/ interpClause i y = true
-                           -> interpClause i (x ++ y) = true.
-  intros; unfold interpClause; rewrite fold_right_app.
-  destruct H.
-  {
-    destruct (fold_right (fun (l : lit) (b : bool) => (interpLit i l || b)%bool)
-                false y); simpl; auto.
-    induction x; simpl in *; auto.
-    destruct (interpLit i a); auto.
-  }
-  {
-    unfold interpClause in H; rewrite H.
-    induction x; simpl; auto.
-    destruct (interpLit i a); auto.
-  }
-Qed.
-  
-Lemma interpFormula_In : forall f i c, interpFormula i f = true
-                                  -> In c f -> interpClause i c = true.
-  induction f; simpl; try tauto; intros.
-  destruct H0; subst.
-  apply Bool.andb_true_iff in H; tauto.
-  apply Bool.andb_true_iff in H; destruct H; auto.
-Qed.
-Hint Resolve interpFormula_In.
-
-Corollary In_entails : forall f c, In c f -> entails f c.
-  unfold entails; intros; eauto 3.
-Qed.
-Hint Resolve In_entails.
-
-
-(*=============================================================================
- * resolvent
- *===========================================================================*)
-
-Theorem eq_lit_dec : forall x y : lit, { x = y } + { x <> y }.
-  decide equality; apply NPeano.Nat.eq_dec.
-Qed.
-
-Definition remove_lit := remove eq_lit_dec.
-  
-Definition resolvent cr c1 c2 v :=
-  let c1' := remove_lit (pos v) c1 in
-  let c2' := remove_lit (neg v) c2 in
-  sublist c1' cr /\ sublist c2' cr.
-
-
-(*=============================================================================
- * resolvent facts
- *===========================================================================*)
-
-Lemma interpClause_drop_lit : forall i l c, interpClause i c = true
-                   -> interpLit i l = false
-                   -> interpClause i (remove_lit l c) = true.
-  induction c; simpl; try congruence; intros.
-  destruct (eq_lit_dec l a); subst.
-  rewrite H0 in H; auto.
-  simpl; destruct (interpLit i a) eqn:?; simpl in *; auto.
-Qed.
-
-Theorem resolvent_sound : forall c1 c2 v i cr, resolvent cr c1 c2 v
-       -> interpClause i c1 = true -> interpClause i c2 = true
-       -> interpClause i cr = true.
-  unfold resolvent; simpl; intros.
-  destruct H.
-  destruct (i v) eqn:?.
-  {
-    eapply interpClause_sublist; try apply H2.
-    apply interpClause_drop_lit; auto.
-    unfold interpLit; rewrite Heqb; auto.
-  }
-  {
-    eapply interpClause_sublist; try apply H.
-    apply interpClause_drop_lit; auto.
-  }
-Qed.
-Hint Resolve resolvent_sound.
-
-Corollary resolvent_entails : forall f c1 c2 v cr, resolvent cr c1 c2 v
-       -> entails f c1 -> entails f c2 -> entails f cr.
-  unfold entails; intros; eauto 4.
-Qed.
-Hint Resolve resolvent_entails.
-
-
-(*=============================================================================
- * Example : (direct) resolution
- *===========================================================================*)
-
-Definition resolve x y v := remove_lit (pos v) x ++ remove_lit (neg v) y.
-
-(* resolve is always is a resolvent *)
-Lemma resolve_resolvent : forall x y v, resolvent (resolve x y v) x y v.
-  unfold resolve, resolvent; split; auto.
-Qed.
-
-Theorem resolve_sound : forall i c1 c2 v,
-       interpClause i c1 = true -> interpClause i c2 = true
-       -> interpClause i (resolve c1 c2 v) = true.
-  intros; eapply resolvent_sound; try apply resolve_resolvent; auto.
-Qed.
-
-
-(*=============================================================================
- * pf
- *===========================================================================*)
-
-Inductive pf (f : formula) : clause -> Prop :=
-| pf_asm c : In c f -> pf f c
-| pf_res cr c1 c2 v : pf f c1 -> pf f c2 -> resolvent cr c1 c2 v -> pf f cr.
-
-Theorem pf_sound : forall f c, pf f c -> entails f c.
-  induction 1; eauto 3.
-Qed.
-Hint Resolve pf_sound.
-
-Lemma pf_nil_interp_false : forall f, pf f nil
-                             -> forall i, interpFormula i f = false.
-  intros.
-  destruct (interpFormula i f) eqn:?; auto.
-  assert (interpClause i nil = true) by (eapply pf_sound; eauto 2).
-  simpl in *; congruence.
-Qed.
-
-Lemma pf_nil_unsat : forall f, pf f nil -> ~ satisfiable f.
-  intros; red; destruct 1.
-  assert (interpFormula x f = false).
-  solve [apply pf_nil_interp_false; auto].
-  congruence.
-Qed.
-
-
-(*=============================================================================
- * todo: pf is refutation complete
- *===========================================================================*)
-
-Conjecture pf_complete : forall f, entails f nil -> pf f nil.
-
-Lemma unsat_pf_nil : forall f, ~ satisfiable f -> pf f nil.
-  intros; apply pf_complete.
-  red; intros.
-  contradict H.
-  red; eauto.
-Qed.
-  
-Theorem dpll_pf : forall n F, wf_formula n F -> dpll n F = None -> pf F nil.
-  intros; apply unsat_pf_nil.
-  eapply dpll_None_sound; eauto 2.
-Qed.
-  
-
-(*=============================================================================
- * denotation into Coq
- *===========================================================================*)
-
-Definition context := list Prop.
-
-Definition denoteLit (g : context) (l : lit) : Prop :=
-  match l with
-    | pos n => nth n g False
-    | neg n => ~ nth n g False
-  end.
-
-Fixpoint denoteClause (g : context) (c : clause) : Prop :=
-  match c with
-    | nil => False
-    | l :: c' => denoteLit g l \/ denoteClause g c'
-  end.
-
-Fixpoint denoteFormula (g : context) f : Prop :=
-  match f with
-    | nil => True
-    | c :: f' => denoteClause g c /\ denoteFormula g f'
-  end.
-
-Lemma denoteFormula_In : forall f g c, denoteFormula g f -> In c f
-                                       -> denoteClause g c.
-  induction f; simpl; try tauto; intros.
-  destruct H, H0; subst; try tauto; auto.
-Qed.
-Hint Resolve denoteFormula_In.
-
-Lemma denoteClause_exists : forall g x, denoteClause g x
-                             -> exists l, In l x /\ denoteLit g l.
-  induction x; simpl; try tauto; intros.
-  destruct H; eauto 4.
-  destruct IHx as [? [] ]; eauto.
-Qed.
-
-Lemma denoteClause_In : forall l g x, denoteLit g l -> In l x
-                                      -> denoteClause g x.
-  induction x; simpl; try tauto; destruct 2; subst; auto.
-Qed.
-Hint Resolve denoteClause_In.
-
-Lemma denoteClause_sublist : forall x g y, denoteClause g x
-                               -> sublist x y -> denoteClause g y.
-  intros.
-  edestruct denoteClause_exists as [? [] ]; eauto 3.
-Qed.
-Hint Resolve denoteClause_sublist.
-
-Lemma denoteClause_remove_lit : forall g l c, denoteClause g c
-               -> denoteClause g (remove_lit l c) \/ denoteLit g l.
-  induction c; simpl; try tauto; destruct 1; subst; auto.
-  {
-    destruct (eq_lit_dec l a); subst; simpl; auto.
-  }
-  {
-    destruct (eq_lit_dec l a); subst; simpl; auto.
-    destruct IHc; auto.
-  }
-Qed.
-
-Lemma denoteLit_contra : forall g v, denoteLit g (pos v) -> denoteLit g (neg v)
-                                     -> False.
-  simpl; tauto.
-Qed.
-Hint Resolve denoteLit_contra.
-
-Lemma denoteClause_resolvent : forall c1 c2 v g cr, resolvent cr c1 c2 v
-                                 -> denoteClause g c1 -> denoteClause g c2
-                                 -> denoteClause g cr.
-  unfold resolvent; destruct 1; intros.
-  edestruct denoteClause_remove_lit; try apply H1; eauto 3.
-  edestruct denoteClause_remove_lit; try apply H2; eauto 3.
-  exfalso; eauto 3.
-Qed.
-Hint Resolve denoteClause_resolvent.
-
-Lemma pf_denote_sound : forall f g c, pf f c -> denoteFormula g f
-                                      -> denoteClause g c.
-  induction 1; intros; eauto 4.
-Qed.
+Section denotation.
+  Variable g : context.
+
+  Definition denoteLit l :=
+    match l with
+      | pos n => g n
+      | neg n => ~ g n
+    end.
+
+  Fixpoint denoteClause c :=
+    match c with
+      | nil => False
+      | l :: c' => denoteLit l \/ denoteClause c'
+    end.
+
+  Fixpoint denoteFormula f :=
+    match f with
+      | nil => True
+      | c :: f' => denoteClause c /\ denoteFormula f'
+    end.
+End denotation.
 
 
 (*=============================================================================
@@ -933,6 +586,7 @@ Fixpoint denoteFormula' (g : context) f : Prop :=
     | c :: f' => denoteClause' g c /\ denoteFormula' g f'
   end.
 
+
 Lemma denoteClause_trim : forall g c, denoteClause' g c -> denoteClause g c.
   induction c; simpl; try tauto; intros.
   destruct c; auto; simpl in *; tauto.
@@ -948,22 +602,45 @@ Lemma denoteFormula_trim : forall g x, denoteFormula' g x -> denoteFormula g x.
 Qed.
 Hint Resolve denoteFormula_trim.
 
-Lemma denoteClause_trim' : forall g c, denoteClause g c -> denoteClause' g c.
-  induction c; simpl; try tauto; intros.
-  destruct H, c; auto; simpl in *; tauto.
-Qed.
 
-Lemma pf_denote_sound' : forall f g c, pf f c -> denoteFormula' g f
-                                       -> denoteClause' g c.
-  intros.
-  apply denoteClause_trim'.
-  eapply pf_denote_sound; eauto 3.
+(*=============================================================================
+ * denoteFormula -> satFormula
+ *===========================================================================*)
+
+Lemma denoteClause_satClause : forall g c, denoteClause g c -> satClause g c.
+  induction c; simpl; try tauto; destruct 1.
+  exists a; simpl; auto.
+  destruct IHc as [? [] ]; auto.
+  exists x; simpl; auto.
 Qed.
+Hint Resolve denoteClause_satClause.
+
+Lemma denoteFormula_satClause : forall g f c, denoteFormula g f -> In c f
+                                              -> satClause g c.
+  induction f; simpl; try tauto; destruct 1, 1; subst; auto.
+Qed.
+Hint Resolve denoteFormula_satClause.
+
+Lemma denoteFormula_satFormula : forall g f, denoteFormula g f -> satFormula g f.
+  red; intros; eauto 3.
+Qed.
+Hint Resolve denoteFormula_satFormula.
 
 
 (*=============================================================================
  * reification
  *===========================================================================*)
+
+Theorem dpll_correct : forall n g f, dpll n f = None -> ~ denoteFormula' g f.
+  red; intros; assert (satFormula g f) by auto.
+  contradict H1; eapply dpll_unsat_sound; eauto.
+Qed.
+
+Corollary dpll_correct' : forall n g f, wf_formula n f -> dpll n f = None
+                                        -> ~ denoteFormula' g f.
+  intros; eapply dpll_correct; eauto.
+Qed.
+
 
 Ltac inList x xs :=
   match xs with
@@ -1030,6 +707,8 @@ Ltac reify :=
       pose f
   end.
 
+Definition nth2fun {A} (l : list A) d := fun n => nth n l d.
+
 
 (*=============================================================================
  * reification tests
@@ -1047,24 +726,31 @@ Section reification_test.
         pose (g:=_g); pose (f:=_f); pose (c:=_c)
     end.
     intro.
-    change (denoteFormula' g f) in H.
-    change (denoteClause' g c).
-    eapply pf_denote_sound'; eauto 3.
-    {
-      constructor; wf.
-    }
-  Qed.
+    change (denoteFormula' (nth2fun g True) f) in H.
+    change (denoteClause' (nth2fun g True) c).
+  Abort.
 End reification_test.
 
 
 (*=============================================================================
- * reflection tests
+ * reflective tactic
  *===========================================================================*)
+
+Ltac dpll_h :=
+  match goal with
+    | |- ~ ?F =>
+      let g := allVars (@nil Prop) F in
+      let f := reifyFormula g F in
+      change (~ denoteFormula' (nth2fun g True) f);
+      apply (dpll_correct (length g)); auto
+  end.
+
+Ltac dpll := solve [dpll_h].
 
 Section PigeonHole.
   Variables p1 p2 p3 p4 p5 p6 p7 p8 p9 p10 p11 p12 : Prop.
 
-  Definition hole2 :=
+  Example hole2 :=
     (~p1 \/ ~p3) /\
     (~p1 \/ ~p5) /\
     (~p3 \/ ~p5) /\
@@ -1075,7 +761,7 @@ Section PigeonHole.
     (p3 \/ p4) /\
     (p5 \/ p6).
 
-  Definition hole3 :=
+  Example hole3 :=
     (~p1 \/ ~p4) /\
     (~p1 \/ ~p7) /\
     (~p1 \/ ~p10) /\
@@ -1102,25 +788,12 @@ Section PigeonHole.
     (p7 \/ p8 \/ p9) /\
     (p10 \/ p11 \/ p12).
 
-  (*Goal hole2 -> False.
-    unfold hole2; tauto.
-  Qed.*)
+  Goal ~ hole2.
+    unfold hole2; dpll.
+  Qed.
 
-  Goal hole3 -> False. (* tauto will be very slow *)
-    unfold hole3.
-    match goal with
-      | |- ?F -> False =>
-        let _g := allVars (@nil Prop) F in
-        let _f := reifyFormula _g F in
-        pose (g:=_g); pose (f:=_f)
-    end.
-    intro H.
-    change (denoteFormula' g f) in H.
-    change (denoteClause' g nil).
-    eapply pf_denote_sound'; eauto 3.
-    assert (wf_formula 12 f) by wf.
-    eapply dpll_pf; try eassumption.
-    compute; auto.
+  Goal ~ hole3. (* tauto will be very slow *)
+    unfold hole3; dpll.
   Qed.
 
 End PigeonHole.
